theories/refinement.v
@@ -362,13 +362,18 @@ Definition malicious_ignore_set (s : NState) (msg : message)
         return [state_prime, lm]
 *)
 Definition process_PrepareBlock_malicious_vote_set (s : NState) (msg : message)
- : NState * list message :=
- let lm := pending_PrepareVote s msg in
- let s' := s
-  <| in_messages := remove message_eq_dec msg s.(in_messages) |>
-  <| counting_messages := msg :: s.(counting_messages) |>
-  <| out_messages := lm ++ s.(out_messages) |>
- in (s', lm).
+ : option (NState * list message) :=
+ match get_quorum_msg_for_block s (parent_of (get_block msg)) with
+ | Some quorum_msg =>
+   let s' := s
+     <| in_messages := remove message_eq_dec msg s.(in_messages) |>
+     <| counting_messages := msg :: s.(counting_messages) |>
+   in
+   let lm := pending_PrepareVote_malicious s' quorum_msg in
+   let s'' := s' <| out_messages := lm ++ s.(out_messages) |>
+   in Some (s'', lm)
+ | None => None
+ end.
 
 (* END STATE UPDATE FUNCTIONS *)
 
@@ -934,17 +939,31 @@ Lemma process_PrepareBlock_malicious_vote_set_eq : forall s msg s' lm,
  get_message_type msg = PrepareBlock ->
  view_valid s msg ->
  exists_same_height_block s (get_block msg) ->
- (process_PrepareBlock_malicious_vote_set s msg = (s',lm) <->
+ (process_PrepareBlock_malicious_vote_set s msg = Some (s',lm) <->
    process_PrepareBlock_malicious_vote s msg s' lm).
 Proof.
 unfold process_PrepareBlock_malicious_vote_set,process_PrepareBlock_malicious_vote.
-split.
-- intros Heq; inversion Heq; subst.
+intros s msg s' lm.
+case_eq (get_quorum_msg_for_block s (parent_of (get_block msg))); split.
+- intros Heq.
+  inversion Heq; subst; clear Heq.
+  apply quorum_msg_for_block_eq in H.
+  exists m; split; [assumption|].
+  split; [reflexivity|].
+  split; [reflexivity|].
   tauto.
 - intros Heq.
-  destruct Heq as [Heq Heq'].
-  destruct Heq' as [Heq' Heq''].
+  destruct Heq as [quorum_msg [Hq Heq]].
+  apply quorum_msg_for_block_eq in Hq.
+  rewrite H in Hq.
+  inversion Hq; subst.
+  destruct Heq as [Hs [Hl Heq]].
   subst; reflexivity.
+- congruence.
+- intros Heq.
+  destruct Heq as [quorum_msg [Hq Heq]].
+  apply quorum_msg_for_block_eq in Hq.
+  congruence.
 Qed.
 
 (* END REFINEMENT PROOFS *)
